Wrote a second, bool-based reflective solver for formulas, but it doesn't work too well. Added formula solver to the procedure for CMon. Put tests for all the solver into separate files.

Reification/CMon.v
@@ -26,11 +26,11 @@ Arguments Id [X].
 Arguments Var [X] _.
 Arguments Op [X] _ _.
 
-Fixpoint expDenote {X : CMon} (env : Env X) (e : exp X) : X :=
+Fixpoint expDenote {X : CMon} (envX : Env X) (e : exp X) : X :=
 match e with
     | Id => neutr
-    | Var n => nth n env neutr
-    | Op e1 e2 => op (expDenote env e1) (expDenote env e2)
+    | Var n => nth n envX neutr
+    | Op e1 e2 => op (expDenote envX e1) (expDenote envX e2)
 end.
 
 Function simplifyExp {X : CMon} (e : exp X) : exp X :=
@@ -46,23 +46,23 @@ match e with
 end.
 
 Theorem simplifyExp_correct :
-  forall (X : CMon) (env : Env X) (e : exp X),
-    expDenote env (simplifyExp e) = expDenote env e.
+  forall (X : CMon) (envX : Env X) (e : exp X),
+    expDenote envX (simplifyExp e) = expDenote envX e.
 Proof.
   intros. functional induction simplifyExp e; cbn;
   rewrite <- ?IHe, <- ?IHe0, <- ?IHe1, ?e3, ?e4; cbn;
   rewrite ?neutr_l, ?neutr_r; trivial.
 Qed.
 
-Fixpoint expDenoteL {X : CMon} (env : Env X) (l : list nat) : X :=
+Fixpoint expDenoteL {X : CMon} (envX : Env X) (l : list nat) : X :=
 match l with
     | [] => neutr
-    | h :: t => op (nth h env neutr) (expDenoteL env t)
+    | h :: t => op (nth h envX neutr) (expDenoteL envX t)
 end.
 
 Lemma expDenoteL_app :
-  forall (X : CMon) (env : Env X) (l1 l2 : list nat),
-    expDenoteL env (l1 ++ l2) = op (expDenoteL env l1) (expDenoteL env l2).
+  forall (X : CMon) (envX : Env X) (l1 l2 : list nat),
+    expDenoteL envX (l1 ++ l2) = op (expDenoteL envX l1) (expDenoteL envX l2).
 Proof.
   induction l1 as [| h1 t1]; simpl; intros.
     rewrite neutr_l. reflexivity.
@@ -70,13 +70,13 @@ Proof.
 Qed.
 
 Lemma expDenoteL_Permutation :
-  forall (X : CMon) (env : Env X) (l1 l2 : list nat),
-    Permutation l1 l2 -> expDenoteL env l1 = expDenoteL env l2.
+  forall (X : CMon) (envX : Env X) (l1 l2 : list nat),
+    Permutation l1 l2 -> expDenoteL envX l1 = expDenoteL envX l2.
 Proof.
   induction 1; cbn.
     reflexivity.
     rewrite IHPermutation. reflexivity.
-    rewrite !assoc. rewrite (comm (nth y env neutr)). reflexivity.
+    rewrite !assoc. rewrite (comm (nth y envX neutr)). reflexivity.
     rewrite IHPermutation1, IHPermutation2. reflexivity.
 Qed.
 
@@ -88,8 +88,8 @@ match e with
 end.
 
 Theorem flatten_correct :
-  forall (X : CMon) (env : Env X) (e : exp X),
-    expDenoteL env (flatten e) = expDenote env e.
+  forall (X : CMon) (envX : Env X) (e : exp X),
+    expDenoteL envX (flatten e) = expDenote envX e.
 Proof.
   induction e; simpl.
     reflexivity.
@@ -98,30 +98,48 @@ Proof.
 Qed.
 
 Theorem sort_correct :
-  forall (X : CMon) (env : Env X) (l : list nat) (s : Sort),
-    expDenoteL env (s natle l) = expDenoteL env l.
+  forall (X : CMon) (envX : Env X) (l : list nat) (s : Sort),
+    expDenoteL envX (s natle l) = expDenoteL envX l.
 Proof.
   intros. apply expDenoteL_Permutation. apply (perm_Permutation natle).
   rewrite <- sort_perm. reflexivity.
 Qed.
 
-Definition simplify {X : CMon} (e : exp X) : list nat :=
-  insertionSort natle (flatten (simplifyExp e)).
+Function list_to_exp {X : CMon} (l : list nat) : exp X :=
+match l with
+    | [] => Id
+    | [x] => Var x
+    | h :: t => Op (Var h) (list_to_exp t)
+end.
+
+Theorem list_to_exp_correct :
+  forall (X : CMon) (envX : Env X) (l : list nat),
+    expDenote envX (list_to_exp l) = expDenoteL envX l.
+Proof.
+  intros. functional induction list_to_exp l; cbn.
+    trivial.
+    rewrite neutr_r. trivial.
+    rewrite IHe. trivial.
+Qed.
+
+Definition simplify {X : CMon} (e : exp X) : exp X :=
+  list_to_exp (insertionSort natle (flatten (simplifyExp e))).
 
 Theorem simplify_correct :
-  forall (X : CMon) (env : Env X) (e : exp X),
-    expDenoteL env (simplify e) = expDenote env e.
+  forall (X : CMon) (envX : Env X) (e : exp X),
+    expDenote envX (simplify e) = expDenote envX e.
 Proof.
   unfold simplify. intros.
+  rewrite !list_to_exp_correct.
   rewrite !(sort_correct _ _ _ Sort_insertionSort).
-  rewrite !flatten_correct, !simplifyExp_correct.
+  erewrite !flatten_correct, !simplifyExp_correct.
   trivial.
 Qed.
 
 Theorem reflectEq :
-  forall (X : CMon) (env : Env X) (e1 e2 : exp X),
-    expDenoteL env (simplify e1) = expDenoteL env (simplify e2) ->
-      expDenote env e1 = expDenote env e2.
+  forall (X : CMon) (envX : Env X) (e1 e2 : exp X),
+    expDenote envX (simplify e1) = expDenote envX (simplify e2) ->
+      expDenote envX e1 = expDenote envX e2.
 Proof.
   intros. rewrite !simplify_correct in H. assumption.
 Qed.
@@ -133,64 +151,430 @@ match e with
     | _ => addToList e xs
 end.
 
-Ltac reifyExp env x :=
+Ltac reifyExp envX x :=
 match x with
     | neutr => constr:(Id)
     | op ?a ?b =>
-        let e1 := reifyExp env a in
-        let e2 := reifyExp env b in constr:(Op e1 e2)
+        let e1 := reifyExp envX a in
+        let e2 := reifyExp envX b in constr:(Op e1 e2)
     | _ =>
-        let n := lookup x env in constr:(Var n)
+        let n := lookup x envX in constr:(Var n)
 end.
 
-Ltac reifyEq env a b :=
-    let e1 := reifyExp env a in
-    let e2 := reifyExp env b in
-      constr:(expDenote env e1 = expDenote env e2).
+Ltac reifyEq envX a b :=
+    let e1 := reifyExp envX a in
+    let e2 := reifyExp envX b in
+      constr:(expDenote envX e1 = expDenote envX e2).
 
-Ltac reflectGoal' := cbn; intros; subst;
+Ltac cmon_simpl := cbn; intros; subst;
 match goal with
     | X : CMon |- ?a = ?b =>
         let xs := allVarsExp constr:(@nil X) b in
         let xs' := allVarsExp xs a in
         let e := reifyEq xs' a b in
-          change e; apply reflectEq; cbn; rewrite ?neutr_l, ?neutr_r
+          change e; apply reflectEq; cbn;
+          rewrite ?neutr_l, ?neutr_r
 end.
 
-Ltac reflectGoal := reflectGoal; reflexivity.
+Ltac cmon := cmon_simpl; reflexivity.
 
-Section Test.
+(* Formulas. [not f] will be represented as [fImpl f fFalse] and
+   [f1 <-> f2] as [fAnd (fImpl f1 f2) (fImpl f2 f1)]. *)
+Inductive formula (X : CMon) : Type :=
+    | fFalse : formula X
+    | fTrue : formula X
+    | fEq : exp X -> exp X -> formula X
+    | fVar : nat -> formula X
+    | fAnd : formula X -> formula X -> formula X
+    | fOr : formula X -> formula X -> formula X
+    | fImpl : formula X -> formula X -> formula X.
 
-Variable (X : CMon) (a a' b b' c c' d e f : X).
+Arguments fFalse [X].
+Arguments fTrue [X].
+Arguments fEq [X] _ _.
+Arguments fVar [X] _.
+Arguments fAnd [X] _ _.
+Arguments fOr [X] _ _.
+Arguments fImpl [X] _ _.
 
-(* [CMon] axioms. *)
-Goal op a (op b c) = op (op a b) c.
-Proof. reflectGoal'. reflexivity. Qed.
+Fixpoint formulaDenote
+  (X : CMon) (envX : Env X) (envP : Env Prop) (f : formula X) : Prop :=
+match f with
+    | fFalse => False
+    | fTrue => True
+    | fVar i => holds i envP
+    | fEq e1 e2 => expDenote envX e1 = expDenote envX e2
+    | fAnd f1 f2 => formulaDenote envX envP f1 /\ formulaDenote envX envP f2
+    | fOr f1 f2 => formulaDenote envX envP f1 \/ formulaDenote envX envP f2
+    | fImpl f1 f2 => formulaDenote envX envP f1 -> formulaDenote envX envP f2
+end.
 
-Goal op neutr a = a.
-Proof. reflectGoal'. reflexivity. Qed.
+Function subst {X : CMon} (e1 : exp X) (n : nat) (e2 : exp X) : exp X :=
+match e1 with
+    | Id => Id
+    | Var m => if Nat.eq_dec n m then e2 else Var m
+    | Op e11 e12 => Op (subst e11 n e2) (subst e12 n e2)
+end.
 
-Goal op a neutr = a.
-Proof. reflectGoal'. reflexivity. Qed.
-
-Goal op a b = op b a.
-Proof. reflectGoal'. reflexivity. Qed.
-
-Goal op a (op (op b c) (op d (op (op e e) d))) =
-     op (op a d) (op d (op c (op e (op e b)))).
-Proof. reflectGoal'. reflexivity. Qed.
-
-(* Other tests. *)
-Goal b = b' -> op a (op b c) = op (op a b') c.
-Proof. reflectGoal'. reflexivity. Qed.
-
-Goal op a b = op a b' -> op (op a b) c = op b' (op a c).
+Theorem subst_correct :
+  forall (X : CMon) (envX : Env X) (envP : Env Prop) (e1 e2 : exp X) (i : nat),
+    formulaDenote envX envP (fEq (Var i) e2) ->
+      expDenote envX (subst e1 i e2) = expDenote envX e1.
 Proof.
-  reflectGoal'. rewrite ?assoc. rewrite (comm b').
-  rewrite <- !H. reflectGoal'. reflexivity.
+  intros. functional induction subst e1 i e2; cbn in *;
+  try rewrite IHe, IHe0; congruence.
 Qed.
 
-Goal a = b -> b = c -> c = a -> op b (op a c) = op a (op neutr (op b c)).
-Proof. reflectGoal'. reflexivity. Qed.
+Function substF {X : CMon} (f : formula X) (i : nat) (e : exp X)
+  : formula X :=
+match f with
+    | fEq e1 e2 => fEq (subst e1 i e) (subst e2 i e)
+    | fAnd f1 f2 => fAnd (substF f1 i e) (substF f2 i e)
+    | fOr f1 f2 => fOr (substF f1 i e) (substF f2 i e)
+    | fImpl f1 f2 => fImpl (substF f1 i e) (substF f2 i e)
+    | _ => f
+end.
 
-End Test.
+Theorem substF_correct :
+  forall (X : CMon) (envX : Env X) (envP : Env Prop) (f : formula X)
+  (i : nat) (e : exp X),
+    (*formulaDenote envX envP (fEq (Var i) e) ->*)
+    nth i envX neutr = expDenote envX e ->
+    formulaDenote envX envP (substF f i e) <-> 
+      formulaDenote envX envP f.
+Proof.
+  intros. functional induction substF f i e; cbn in *.
+    rewrite !(@subst_correct _ envX envP); cbn; firstorder.
+    all: firstorder.
+Qed.
+
+Function simplifyFormula {X : CMon} (f : formula X) : formula X :=
+match f with
+    | fFalse => fFalse
+    | fTrue => fTrue
+    | fVar P => fVar P
+    | fEq e1 e2 => fEq (simplify e1) (simplify e2)
+    | fAnd f1 f2 =>
+        match simplifyFormula f1, simplifyFormula f2 with
+            | fOr f11 f12, f2' => fOr (fAnd f11 f2') (fAnd f12 f2')
+            | f1', fOr f21 f22 => fOr (fAnd f1' f21) (fAnd f1' f22)
+            | fFalse, _ => fFalse
+            | _, fFalse => fFalse
+            | fTrue, f2' => f2'
+            | f1', fTrue => f1'
+            | f1', f2' => fAnd f1' f2'
+        end
+    | fOr f1 f2 =>
+        match simplifyFormula f1, simplifyFormula f2 with
+            | fAnd f11 f12, f2' => fAnd (fOr f11 f2') (fOr f12 f2')
+            | f1', fAnd f21 f22 => fAnd (fOr f1' f21) (fOr f1' f22)
+            | fFalse, f2' => f2'
+            | f1', fFalse => f1'
+            | fTrue, _ => fTrue
+            | _, fTrue => fTrue
+            | f1', f2' => fOr f1' f2'
+        end
+    | fImpl f1 f2 =>
+        let f2' := simplifyFormula f2 in
+        match simplifyFormula f1 with
+            | fFalse => fTrue
+            | fTrue => f2'
+            | fEq (Var i) e => fImpl (fEq (Var i) e) (substF f2' i e)
+            | fAnd f11 f12 => fImpl f11 (fImpl f12 f2')
+            | fOr f11 f12 => fAnd (fImpl f11 f2') (fImpl f12 f2')
+            | f1' => fImpl f1' f2'
+        end
+end.
+
+(*Fixpoint simpHyp {X : CMon} (hyp goal : formula X) : formula X :=
+match hyp with
+    | fFalse => fTrue
+    | fTrue => simpGoal goal
+    | fEq (Var i) e => fImpl (fEq (Var i) e) (simpGoal (substF goal i e))
+    | fAnd f11 f12 => fImpl f11 (fImpl f12 (simpGoal goal))
+    | fOr f11 f12 => fAnd (fImpl f11 (simpGoal goal)) (fImpl f12 (simpGoal goal))
+    | f1' => fImpl f1' (simpGoal goal)
+end
+
+with simpGoal {X : CMon} (f : formula X) : formula X := f.
+
+Fixpoint size {X : CMon} (f : formula X) : nat :=
+match f with
+    | fFalse => 1
+    | fTrue => 1
+    | fEq _ _ => 1
+    | fVar _ => 1
+    | fAnd f1 f2 => size f1 + size f2
+    | fOr f1 f2 => size f1 + size f2
+    | fImpl f1 f2 => size f1 + size f2
+end.
+
+Lemma size_gt_0 :
+  forall (X : CMon) (f : formula X), 0 < size f.
+Proof.
+  induction f; cbn; omega.
+Qed.
+
+Lemma size_substF :
+  forall (X : CMon) (f : formula X) (i : nat) (e : exp X),
+    size (substF f i e) = size f.
+Proof.
+  intros. functional induction substF f i e; cbn; omega.
+Qed.
+
+Require Import Recdef.
+Require Import Coq.Program.Wf.
+
+Hint Resolve size_gt_0.
+
+Program Fixpoint simp {X : CMon} (f : formula X) {measure (size f)}
+  : formula X :=
+match f with
+    | fFalse => fFalse
+    | fTrue => fTrue
+    | fVar P => fVar P
+    | fEq e1 e2 => fEq (simplify e1) (simplify e2)
+    | fAnd f1 f2 =>
+        match simp f1, simp f2 with
+            | fOr f11 f12, f2' => fOr (fAnd f11 f2') (fAnd f12 f2')
+            | f1', fOr f21 f22 => fOr (fAnd f1' f21) (fAnd f1' f22)
+            | fFalse, _ => fFalse
+            | _, fFalse => fFalse
+            | fTrue, f2' => f2'
+            | f1', fTrue => f1'
+            | f1', f2' => fAnd f1' f2'
+        end
+    | fOr f1 f2 =>
+        match simp f1, simp f2 with
+            | fAnd f11 f12, f2' => fAnd (fOr f11 f2') (fOr f12 f2')
+            | f1', fAnd f21 f22 => fAnd (fOr f1' f21) (fOr f1' f22)
+            | fFalse, f2' => f2'
+            | f1', fFalse => f1'
+            | fTrue, _ => fTrue
+            | _, fTrue => fTrue
+            | f1', f2' => fOr f1' f2'
+        end
+    | fImpl f1 f2 =>
+        let f2' := simp f2 in
+        match simp f1 with
+            | fFalse => fTrue
+            | fTrue => f2'
+            | fEq (Var i) e =>
+                fImpl (fEq (Var i) e) (simp (substF f2 i e))
+            | fAnd f11 f12 => fImpl f11 (fImpl f12 f2')
+            | fOr f11 f12 => fAnd (fImpl f11 f2') (fImpl f12 f2')
+            | f1' => fImpl f1' f2'
+        end
+end.
+Obligation Tactic := intros; subst; cbn;
+match goal with
+    | f1 : formula _, f2 : formula _ |- _ =>
+        pose (size_gt_0 f1); pose (size_gt_0 f2); try omega
+end.
+Solve All Obligations.
+Next Obligation. firstorder.
+  
+  try pose (size_gt_0 f1); try pose (size_gt_0 f2); try omega.
+    rewrite size_substF. omega.
+Defined.*)
+
+Theorem simplifyFormula_correct :
+  forall (X : CMon) (f : formula X) (envX : Env X) (envP : Env Prop),
+    formulaDenote envX envP (simplifyFormula f) <-> formulaDenote envX envP f.
+Proof.
+  intros. functional induction simplifyFormula f; cbn.
+  Time all:
+  repeat match goal with
+      | envX : Env _, IH : forall _ : Env _, _ |- _ => specialize (IH envX)
+      | e : simplifyFormula ?f = _,
+        IH : formulaDenote _ _ (simplifyFormula ?f) <-> _ |- _ =>
+        rewrite <- IH, e; cbn
+  end; try (tauto; fail).
+    rewrite !simplify_correct. tauto.
+    rewrite e1 in IHf1. cbn in *. rewrite IHf1. split; intros.
+      rewrite <- IHf0. rewrite <- substF_correct.
+        apply H. assumption.
+        rewrite IHf1. assumption.
+      rewrite substF_correct.
+        rewrite IHf0. apply H. assumption.
+        rewrite IHf1. assumption.
+Qed.
+
+Definition solveEq
+  {X : CMon} (envX : Env X) (envP : Env Prop)
+    : forall e1 e2 : exp X, solution (formulaDenote envX envP (fEq e1 e2)).
+Proof.
+  refine (
+  fix solve (e1 e2 : exp X)
+    : solution (formulaDenote envX envP (fEq e1 e2)) :=
+  match e1, e2 with
+      | Id, Id => Yes
+      | Var n, Var m => if Nat.eq_dec n m then Yes else No
+      | Op e11 e12, Op e21 e22 => solve e11 e21 && solve e12 e22
+      | _, _ => No
+  end);
+  cbn in *; congruence.
+Defined.
+
+Definition solveHypothesis {X : CMon} (envX : Env X) (envP : Env Prop) :
+  forall (proofs : Proofs) (hyp f : formula X)
+    (cont : forall proofs : Proofs,
+      solution (allTrue envP proofs -> formulaDenote envX envP f)),
+        solution (allTrue envP proofs -> formulaDenote envX envP hyp ->
+          formulaDenote envX envP f).
+Proof.
+  refine (
+  fix solve
+    (proofs : Proofs) (hyp f : formula X)
+      (cont : forall proofs : Proofs,
+        solution (allTrue envP proofs -> formulaDenote envX envP f)) :
+          solution (allTrue envP proofs -> formulaDenote envX envP hyp ->
+            formulaDenote envX envP f) :=
+  match hyp with
+      | fFalse => Yes
+      | fTrue => Reduce (cont proofs)
+      | fVar i => Reduce (cont (i :: proofs))
+      (*| fEq (Var i) e => Reduce (cont proofs)*)
+      | fEq _ _ => Reduce (cont proofs)
+      | fAnd f1 f2 =>
+          Reduce (solve proofs f1 (fImpl f2 f)
+                        (fun proofs' => Reduce (cont proofs')))
+      | fOr f1 f2 =>
+          solve proofs f1 f cont &&
+          solve proofs f2 f cont
+      | _ => No
+  end).
+  all: cbn in *; try tauto.
+Defined.
+
+Definition solveGoal {X : CMon} (envX : Env X) (envP : Env Prop)
+  : forall (proofs : Proofs) (f : formula X),
+      solution (allTrue envP proofs -> formulaDenote envX envP f).
+Proof.
+  refine (
+  fix solve
+    (proofs : Proofs) (f : formula X)
+      : solution (allTrue envP proofs -> formulaDenote envX envP f) :=
+  match f with
+      | fFalse => No
+      | fTrue => Yes
+      | fVar i =>
+          match in_dec Nat.eq_dec i proofs with
+              | left _ => Yes
+              | right _ => No
+          end
+      | fEq e1 e2 => Reduce (solveEq envX envP e1 e2)
+      | fAnd f1 f2 => solve proofs f1 && solve proofs f2
+      | fOr f1 f2 => solve proofs f1 || solve proofs f2
+      | fImpl f1 f2 =>
+          solveHypothesis envX envP proofs f1 f2
+            (fun proofs' => solve proofs' f2)
+  end).
+  all: cbn; try tauto.
+    intro. apply find_spec with proofs; assumption.
+Defined.
+
+Definition solveFormula
+  {X : CMon} (envX : Env X) (envP : Env Prop) (f : formula X)
+    : solution (formulaDenote envX envP f).
+Proof.
+  refine (Reduce (solveGoal envX envP [] f)). apply f0. cbn. trivial.
+Defined.
+
+Theorem solveFormula_correct :
+  forall (X : CMon) (envX : Env X) (envP : Env Prop) (f : formula X),
+    (exists p : formulaDenote envX envP f,
+      solveFormula envX envP f = Yes' p) ->
+        formulaDenote envX envP f.
+Proof.
+  intros. destruct H. assumption.
+Qed.
+
+Ltac allVarsX xs P :=
+match P with
+    | False => xs
+    | True => xs
+    | ?a = ?b =>
+        let xs' := allVarsExp xs b in allVarsExp xs' a
+    | ~ ?P' => allVarsX xs P'
+    | ?P1 /\ ?P2 =>
+        let xs' := allVarsX xs P2 in allVarsX xs' P1
+    | ?P1 \/ ?P2 =>
+        let xs' := allVarsX xs P2 in allVarsX xs' P1
+    | ?P1 -> ?P2 =>
+        let xs' := allVarsX xs P2 in allVarsX xs' P1
+    | ?P1 <-> ?P2 =>
+        let xs' := allVarsX xs P2 in allVarsX xs' P1
+    | _ =>
+        match type of P with
+            | Prop => xs
+            | _ => addToList P xs
+        end
+end.
+
+Ltac allVarsProp xs P :=
+match P with
+    | False => xs
+    | True => xs
+    | ?a = ?b => xs
+    | ~ ?P' => allVarsProp xs P'
+    | ?P1 /\ ?P2 =>
+        let xs' := allVarsProp xs P2 in allVarsProp xs' P1
+    | ?P1 \/ ?P2 =>
+        let xs' := allVarsProp xs P2 in allVarsProp xs' P1
+    | ?P1 -> ?P2 =>
+        let xs' := allVarsProp xs P2 in allVarsProp xs' P1
+    | ?P1 <-> ?P2 =>
+        let xs' := allVarsProp xs P2 in allVarsProp xs' P1
+    | _ => addToList P xs
+end.
+
+Ltac reifyFormula envX envP P :=
+match P with
+    | False => constr:(fFalse)
+    | True => constr:(fTrue)
+    | ?a = ?b =>
+        let e1 := reifyExp envX a in
+        let e2 := reifyExp envX b in constr:(fEq e1 e2)
+    | ~ ?P' =>
+        let e := reifyFormula envX envP P' in constr:(fImpl e fFalse)
+    | ?P1 /\ ?P2 =>
+        let e1 := reifyFormula envX envP P1 in
+        let e2 := reifyFormula envX envP P2 in constr:(fAnd e1 e2)
+    | ?P1 \/ ?P2 =>
+        let e1 := reifyFormula envX envP P1 in
+        let e2 := reifyFormula envX envP P2 in constr:(fOr e1 e2)
+    | ?P1 -> ?P2 =>
+        let e1 := reifyFormula envX envP P1 in
+        let e2 := reifyFormula envX envP P2 in constr:(fImpl e1 e2)
+    | ?P1 <-> ?P2 =>
+        let e1 := reifyFormula envX envP P1 in
+        let e2 := reifyFormula envX envP P2 in
+          constr:(fAnd (fImpl e1 e2) (fImpl e2 e1))
+    | _ =>
+        let i := lookup P envP in constr:(fVar i)
+end.
+
+Ltac solveGoal' X :=
+match goal with
+    | |- ?P =>
+        let envX := allVarsX constr:(@nil X) P in
+        let envP := allVarsProp constr:(@nil Prop) P in
+        let f := reifyFormula envX envP P in
+          change (formulaDenote envX envP f);
+          rewrite <- simplifyFormula_correct; cbn;
+          try apply (unwrap (solveFormula envX envP (simplifyFormula f)))
+end.
+
+Instance CMon_unit : CMon :=
+{
+    carrier := unit;
+    op := fun _ _ => tt
+}.
+Proof. all: try destruct x; firstorder. Defined.
+
+Ltac solveGoal := do 2
+match goal with
+    | X : CMon |- ?P => solveGoal' X
+    | |- ?P => solveGoal' CMon_unit
+end.
