Reification/CMon2.v
@@ -28,11 +28,9 @@ Inductive exp {X : CMon} : type X -> Type :=
     | Id : exp elem
     | Var : nat -> exp elem
     | Op : exp elem -> exp elem -> exp elem
-(*    | fVar : nat -> exp prop*)
     | fFalse : exp prop
     | fTrue : exp prop
     | fEquiv : exp elem -> exp elem -> exp prop
-(*    | fNot : exp prop -> exp prop*)
     | fAnd : exp prop -> exp prop -> exp prop
     | fOr : exp prop -> exp prop -> exp prop
     | fImpl : exp prop -> exp prop -> exp prop.
@@ -40,9 +38,7 @@ Inductive exp {X : CMon} : type X -> Type :=
 Arguments Id [X].
 Arguments Var [X] _.
 Arguments Op [X] _ _.
-(*Arguments fVar [X] _.*)
 Arguments fEquiv [X] _ _.
-(*Arguments fNot [X] _.*)
 Arguments fAnd [X] _ _.
 Arguments fOr [X] _ _.
 Arguments fImpl [X] _ _.
@@ -59,11 +55,9 @@ match f with
     | Id => neutr
     | Var n => nth n env neutr
     | Op e1 e2 => op (denote env e1) (denote env e2)
-(*    | fVar i => nth i False*)
     | fFalse => False
     | fTrue => True
     | fEquiv e1 e2 => denote env e1 = denote env e2
-(*    | fNot f' => ~ denote env f'*)
     | fAnd f1 f2 => denote env f1 /\ denote env f2
     | fOr f1 f2 => denote env f1 \/ denote env f2
     | fImpl f1 f2 => denote env f1 -> denote env f2
@@ -147,14 +141,32 @@ Proof.
   rewrite <- sort_perm. reflexivity.
 Qed.
 
-Definition simplify {X : CMon} (e : exp elem) : list nat :=
-  insertionSort natle (flatten (simplifyExp e)).
+Function list_to_exp {X : CMon} (l : list nat) : exp elem :=
+match l with
+    | [] => Id
+    | [x] => Var x
+    | h :: t => Op (Var h) (list_to_exp t)
+end.
+
+Theorem list_to_exp_correct :
+  forall (X : CMon) (env : Env X) (l : list nat),
+    denote env (list_to_exp l) = denoteL env l.
+Proof.
+  intros. functional induction list_to_exp l; cbn.
+    trivial.
+    rewrite neutr_r. trivial.
+    rewrite IHe. trivial.
+Qed.
+
+Definition simplify {X : CMon} (e : exp elem) : exp elem :=
+  list_to_exp (insertionSort natle (flatten (simplifyExp e))).
 
 Theorem simplify_correct :
   forall (X : CMon) (env : Env X) (e : exp elem),
-    denoteL env (simplify e) = denote env e.
+    denote env (simplify e) = denote env e.
 Proof.
   unfold simplify. intros.
+  rewrite !list_to_exp_correct.
   rewrite !(sort_correct _ _ _ Sort_insertionSort).
   erewrite !flatten_correct, !simplifyExp_correct.
   trivial.
@@ -162,94 +174,11 @@ Qed.
 
 Theorem reflectEq :
   forall (X : CMon) (env : Env X) (e1 e2 : exp elem),
-    denoteL env (simplify e1) = denoteL env (simplify e2) ->
+    denote env (simplify e1) = denote env (simplify e2) ->
       denote env e1 = denote env e2.
 Proof.
   intros. rewrite !simplify_correct in H. assumption.
 Qed.
-
-Ltac allVarsExp xs e :=
-match e with
-    | op ?e1 ?e2 =>
-        let xs' := allVarsExp xs e2 in allVarsExp xs' e1
-    | _ => addToList e xs
-end.
-
-Ltac reifyExp env x :=
-match x with
-    | neutr => constr:(Id)
-    | op ?a ?b =>
-        let e1 := reifyExp env a in
-        let e2 := reifyExp env b in constr:(Op e1 e2)
-    | _ =>
-        let n := lookup x env in constr:(Var n)
-end.
-
-Ltac reifyEq env a b :=
-    let e1 := reifyExp env a in
-    let e2 := reifyExp env b in
-      constr:(denote env e1 = denote env e2).
-
-Ltac reflectGoal' := cbn; intros; subst;
-match goal with
-    | X : CMon |- ?a = ?b =>
-        let xs := allVarsExp constr:(@nil X) b in
-        let xs' := allVarsExp xs a in
-        let e := reifyEq xs' a b in
-          change e; apply reflectEq; cbn; rewrite ?neutr_l, ?neutr_r
-end.
-
-Ltac reflectGoal := reflectGoal; reflexivity.
-
-Ltac allVarsFormula xs P :=
-match P with
-    | ?a = ?b =>
-        let xs' := allVarsExp xs b in allVarsExp xs' a
-    | ?P1 /\ ?P2 =>
-        let xs' := allVarsFormula xs P2 in allVarsFormula xs' P1
-    | ?P1 \/ ?P2 =>
-        let xs' := allVarsFormula xs P2 in allVarsFormula xs' P1
-    | ?P1 -> ?P2 =>
-        let xs' := allVarsFormula xs P2 in allVarsFormula xs' P1
-    | ?P1 <-> ?P2 =>
-        let xs' := allVarsFormula xs P2 in allVarsFormula xs' P1
-    | _ => xs
-end.
-
-Ltac reifyFormula xs P :=
-match P with
-    | ?a = ?b =>
-        let e1 := reifyExp xs a in
-        let e2 := reifyExp xs b in constr:(fEquiv e1 e2)
-    | ~ ?P' =>
-        let e := reifyFormula xs P' in constr:(fImpl e fFalse)
-    | ?P1 /\ ?P2 =>
-        let e1 := reifyFormula xs P1 in
-        let e2 := reifyFormula xs P2 in constr:(fAnd e1 e2)
-    | ?P1 \/ ?P2 =>
-        let e1 := reifyFormula xs P1 in
-        let e2 := reifyFormula xs P2 in constr:(fOr e1 e2)
-    | ?P1 -> ?P2 =>
-        let e1 := reifyFormula xs P1 in
-        let e2 := reifyFormula xs P2 in constr:(fImpl e1 e2)
-    | ?P1 <-> ?P2 =>
-        let e1 := reifyFormula xs P1 in
-        let e2 := reifyFormula xs P2 in
-          constr:(fAnd (fImpl e1 e2) (fImpl e2 e1))
-end.
-
-Ltac reifyGoal :=
-match goal with
-    | X : CMon |- ?P =>
-        let xs := allVarsFormula constr:(@nil X) P in
-        let e := reifyFormula xs P in change (denote xs e)
-end.
-
-Definition list_eq :
-  forall (l1 l2 : list nat), {l1 = l2} + {l1 <> l2}.
-Proof.
-  do 2 decide equality.
-Defined.
 
 Fixpoint solve
   {X : CMon} (env : Env X) (f : exp prop)
@@ -258,11 +187,7 @@ Proof.
   dependent destruction f; cbn.
     apply None.
     apply Some. trivial.
-    destruct (list_eq
-              (insertionSort natle (flatten (simplifyExp f1)))
-              (insertionSort natle (flatten (simplifyExp f2)))).
-      apply Some. apply reflectEq. f_equal. assumption.
-      apply None.
+    apply None.
     destruct (solve X env f1), (solve X env f2).
       apply Some. split; assumption.
       1-3: apply None.
@@ -284,58 +209,96 @@ Proof.
   intros. destruct H. assumption.
 Qed.
 
-Axiom JMeq_eq_refl :
-  forall (A : Type) (x : A) (p : x ~= x),
-    @JMeq_eq A x x p = eq_refl x.
+Definition simplifyFormula {X : CMon} (t : type X) : exp t -> exp t :=
+match t with
+    | elem => fun e => simplify e
+    | prop => fun e =>
+        match e with
+            | fEquiv e1 e2 => fEquiv (simplify e1) (simplify e2)
+            | _ => e
+        end
+end.
 
-(*Ltac solve_goal' :=
-  cbn; intros; cmon_subst; reifyGoal; apply solve_spec;
-  repeat (try eexists; compute; rewrite ?JMeq_eq_refl); eauto.
-
-Ltac solve_goal :=
-  try (solve_goal'; fail);
-  fail "Cannot solve the goal".*)
-
-Section Test.
-
-Variable (X : CMon) (a a' b b' c c' d e f : X).
-
-(* [CMon] axioms. *)
-Goal op a (op b c) = op (op a b) c.
-Proof. reflectGoal'. reflexivity. Qed.
-
-Goal op neutr a = a.
-Proof. reflectGoal'. reflexivity. Qed.
-
-Goal op a neutr = a.
-Proof. reflectGoal'. reflexivity. Qed.
-
-Goal op a b = op b a.
-Proof. reflectGoal'. reflexivity. Qed.
-
-Goal op a (op (op b c) (op d (op (op e e) d))) =
-     op (op a d) (op d (op c (op e (op e b)))).
-Proof. reflectGoal'. reflexivity. Qed.
-
-(* Other tests. *)
-Goal b = b' -> op a (op b c) = op (op a b') c.
-Proof. reflectGoal'. reflexivity. Qed.
-
-Goal op a b = op a b' -> op (op a b) c = op b' (op a c).
+Theorem simplifyFormula_correct :
+  forall (X : CMon) (t : type X) (env : Env X) (e : exp t),
+    denote env (simplifyFormula e) = denote env e.
 Proof.
-  reflectGoal'. rewrite ?assoc. rewrite (comm b').
-  rewrite <- !H. reflectGoal'. reflexivity.
+  destruct t; cbn; intros.
+    rewrite simplify_correct. trivial.
+    dependent destruction e; trivial.
+      cbn. rewrite !simplify_correct. trivial.
 Qed.
 
-Goal a = b -> b = c -> c = a -> op b (op a c) = op a (op neutr (op b c)).
-Proof. reflectGoal'. reflexivity. Qed.
-
-(* Tests for formulas. *)
-Goal a = b -> b = c -> c = a -> a = c /\ op c c = op b b.
+Theorem reflectFormula :
+  forall (X : CMon) (env : Env X) (e : exp prop),
+    denote env (simplifyFormula e) -> denote env e.
 Proof.
-  intros. split.
-    reflectGoal'. reflexivity.
-    reflectGoal'. reflexivity. 
+  dependent induction e; cbn; trivial.
+    rewrite !simplify_correct. trivial.
 Qed.
 
-End Test.
+Ltac allVars X xs e :=
+match e with
+    | op ?e1 ?e2 =>
+        let xs' := allVars X xs e2 in allVars X xs' e1
+    | ?a = ?b =>
+        let xs' := allVars X xs b in allVars X xs' a
+    | ~?P => allVars xs P
+    | ?P1 /\ ?P2 =>
+        let xs' := allVars X xs P2 in allVars X xs' P1
+    | ?P1 \/ ?P2 =>
+        let xs' := allVars X xs P2 in allVars X xs' P1
+    | ?P1 -> ?P2 =>
+        let xs' := allVars X xs P2 in allVars X xs' P1
+    | ?P1 <-> ?P2 =>
+        let xs' := allVars X xs P2 in allVars X xs' P1
+    | _ =>
+        match type of e with
+            | X => addToList e xs
+        end
+end.
+
+Ltac reify env e :=
+match e with
+    | neutr => constr:(Id)
+    | op ?a ?b =>
+        let e1 := reify env a in
+        let e2 := reify env b in constr:(Op e1 e2)
+    | False => constr:(fFalse)
+    | True => constr:(fTrue)
+    | ?a = ?b =>
+        let e1 := reify env a in
+        let e2 := reify env b in constr:(fEquiv e1 e2)
+    | ~?P =>
+        let e' := reify env P in constr:(fImpl e' fFalse)
+    | ?P1 /\ ?P2 =>
+        let e1 := reify env P1 in
+        let e2 := reify env P2 in constr:(fAnd e1 e2)
+    | ?P1 \/ ?P2 =>
+        let e1 := reify env P1 in
+        let e2 := reify env P2 in constr:(fOr e1 e2)
+    | ?P1 -> ?P2 =>
+        let e1 := reify env P1 in
+        let e2 := reify env P2 in constr:(fImpl e1 e2)
+    | ?P1 <-> ?P2 =>
+        let e1 := reify env P1 in
+        let e2 := reify env P2 in constr:(fAnd (fImpl e1 e2) (fImpl e2 e1))
+    | _ =>
+        let n := lookup e env in constr:(Var n)
+end.
+
+Ltac reflectGoal :=
+match goal with
+    | X : CMon |- ?P =>
+        let env := allVars (@carrier X) constr:(@nil X) P in
+        let e := reify env P in
+          change (denote env e);
+          apply reflectFormula; cbn
+end.
+
+Ltac cmon_simpl := cbn; intros; subst;
+match goal with
+    | X : CMon |- ?a = ?b => reflectGoal
+end.
+
+Ltac cmon := cmon_simpl; reflexivity.
