Reification/ReificationBase.v
@@ -34,3 +34,44 @@ match l with
 end.
 
 Definition Env (X : Type) : Type := list X.
+
+Definition holds (n : nat) (env : Env Prop) : Prop := nth n env False.
+
+Definition Proofs : Type := list nat.
+
+Fixpoint allTrue (env : Env Prop) (proofs : Proofs) : Prop :=
+match proofs with
+    | [] => True
+    | h :: t => holds h env /\ allTrue env t
+end.
+
+Theorem find_spec :
+  forall (n : nat) (env : Env Prop) (proofs : Proofs),
+    allTrue env proofs -> In n proofs -> holds n env.
+Proof.
+  induction proofs as [| h t]; cbn.
+    inversion 2.
+    do 2 destruct 1; subst.
+      unfold holds in H. apply H.
+      apply IHt; assumption.
+Qed.
+
+Inductive solution (P : Prop) : Type :=
+    | Yes' : P -> solution P
+    | No' : solution P.
+
+Arguments Yes' [P] _.
+Arguments No' [P].
+
+Notation "'Yes'" := (Yes' _).
+Notation "'No'" := No'.
+
+Notation "'Reduce' x" := (if x then Yes else No) (at level 50).
+Notation "x && y" := (if x then Reduce y else No).
+Notation "x || y" := (if x then Yes else Reduce y).
+
+Definition unwrap {P : Prop} (s : solution P) :=
+match s return if s then P else Prop with
+    | Yes' p => p
+    | _ => True
+end.
