Reification/CMonTest.v
@@ -1,0 +1,39 @@
+Add Rec LoadPath "/home/zeimer/Code/Coq".
+
+Require Import CMon.
+
+Section Test.
+
+Variable (X : CMon) (a a' b b' c c' d e f : X).
+
+(* [CMon] axioms. *)
+Goal op a (op b c) = op (op a b) c.
+Proof. cmon_simpl. reflexivity. Qed.
+
+Goal op neutr a = a.
+Proof. cmon_simpl. reflexivity. Qed.
+
+Goal op a neutr = a.
+Proof. cmon_simpl. reflexivity. Qed.
+
+Goal op a b = op b a.
+Proof. cmon_simpl. reflexivity. Qed.
+
+Goal op a (op (op b c) (op d (op (op e e) d))) =
+     op (op a d) (op d (op c (op e (op e b)))).
+Proof. cmon_simpl. reflexivity. Qed.
+
+(* Other tests. *)
+Goal b = b' -> op a (op b c) = op (op a b') c.
+Proof. solveGoal. Qed.
+
+Goal op a b = op a b' -> op (op a b) c = op b' (op a c).
+Proof.
+  cmon_simpl. rewrite ?assoc. rewrite (comm b').
+  rewrite <- !H. cmon_simpl. reflexivity.
+Qed.
+
+Goal a = b -> b = c -> c = a -> op b (op a c) = op a (op neutr (op b c)).
+Proof. cmon_simpl. reflexivity. Qed.
+
+End Test.
